{
 "cells": [
  {
   "cell_type": "markdown",
   "metadata": {},
   "source": [
    "**Jonathan Remiere Inso BSCS - 1B CIS 1203**"
   ]
  },
  {
   "cell_type": "markdown",
   "metadata": {
    "vscode": {
     "languageId": "latex"
    }
   },
   "source": [
    "*1. Recall the definition of a rational number, denoted as $\\mathbb{Q}$. Prove that Euler's number $e = \\sum_{k=0}^\\infty \\frac{1}{k!} \\notin \\mathbb{Q}$. A factorial is defined as $k! = (k)(k-1)(k-2)(k-3)..., \\forall k \\in \\mathbb{Z}^+$, note that $0! = 1$. Furthermore, a sum notation $\\sum_{k=0}^\\infty k = 0+ 1 + 2 + 3 +....+...$.*\n",
    "<br><br>\n",
    "\n",
    "**ANSWER:**\n",
    "\n",
    "\n",
    "Step 1:\n",
    "\n",
    "To demonstrate that Euler's constant $e$ is irrational, we'll use proof by contradiction.\n",
    "\n",
    "Let's assume that $e$ is rational, meaning it can be represented as the fraction of two integers $p$ and $q$, where $q \\neq 0$. Hence, $e = \\frac{p}{q}$.\n",
    "\n",
    "Recall the definition of $e$: \n",
    "\n",
    "$ e = \\frac{1}{0!} + \\frac{1}{1!} + \\frac{1}{2!} + \\frac{1}{3!} + \\ldots $\n",
    "\n",
    "Step 2:\n",
    "\n",
    "Consider the partial sum of the series:\n",
    "\n",
    "$ S_n = \\frac{1}{0!} + \\frac{1}{1!} + \\frac{1}{2!} + \\frac{1}{3!} + \\ldots + \\frac{1}{n!} $\n",
    "\n",
    "for some positive integer $n$. As each term in the series is positive, $S_n$ increases and is bounded above by $e$, thus converging to $e$ as $n$ approaches infinity.\n",
    "\n",
    "Step 3:\n",
    "\n",
    "Consider the expression:\n",
    "\n",
    "$ q! \\cdot S_n = q! \\cdot \\left(\\frac{1}{0!} + \\frac{1}{1!} + \\frac{1}{2!} + \\frac{1}{3!} + \\ldots + \\frac{1}{n!}\\right) $\n",
    "\n",
    "Step 4:\n",
    "\n",
    "Expand:\n",
    "\n",
    "$ q! \\cdot S_n = q! + \\frac{q!}{1!} + \\frac{q!}{2!} + \\frac{q!}{3!} + \\ldots + \\frac{q!}{n!} $\n",
    "\n",
    "Step 5:\n",
    "\n",
    "Every term in this expression is an integer. Since $S_n$ converges to $e$, $q! \\cdot S_n$ should be very close to $q! \\cdot e = p$. This suggests that $p - q! \\cdot S_n$ should be a very small positive integer.\n",
    "\n",
    "$ p - q! \\cdot S_n = p - (q! + \\frac{q!}{1!} + \\frac{q!}{2!} + \\frac{q!}{3!} + \\ldots + \\frac{q!}{n!}) $\n",
    "\n",
    "$ p - q! \\cdot S_n = p - q! - \\frac{q!}{1!} - \\frac{q!}{2!} - \\frac{q!}{3!} - \\ldots - \\frac{q!}{n!} $\n",
    "\n",
    "$ p - q! \\cdot S_n = (p - q!) - \\frac{q!}{1!} - \\frac{q!}{2!} - \\frac{q!}{3!} - \\ldots - \\frac{q!}{n!} $\n",
    "\n",
    "Step 6:\n",
    "\n",
    "Every number enclosed in the brackets is a whole number, and every number within the sum is a fraction with a denominator larger than 1. Therefore, the expression $p - q! \\cdot S_n$ has to be a positive whole number that isn't zero.\n",
    "\n",
    "Nevertheless, this conflicts with the assertion that $e = \\frac{p}{q}$ because $q! \\cdot S_n$ should closely approach $p$ but does not match it precisely, resulting in a contradiction.\n",
    "\n",
    "<br>\n",
    "\n",
    "**So, our presumption that $e$ is rational is wrong, thus establishing that $e$ is irrational.**\n",
    "\n",
    "<br>\n",
    "\n",
    "****"
   ]
  },
  {
   "cell_type": "markdown",
   "metadata": {},
   "source": [
    "*2. Prove Minkowski's Inequality for sums, $\\forall \\ p>1, (a_k, b_k)>0$:*\n",
    "\n",
    "\\begin{gather}\n",
    "\\begin{bmatrix}\n",
    "\\sum_{k=1}^n |a_k + b_k|^p\n",
    "\\end{bmatrix}^\\frac{1}{p}\n",
    "\\leq\n",
    "\\begin{bmatrix}\n",
    "\\sum_{k=1}^n |a_k|^p\n",
    "\\end{bmatrix}^\\frac{1}{p}\n",
    "+\n",
    "\\begin{bmatrix}\n",
    "\\sum_{k=1}^n |b_k|^p\n",
    "\\end{bmatrix}^\\frac{1}{p}\n",
    "\\end{gather}\n",
    "\n",
    "<br><br>\n",
    "**ANSWER:**\n",
    "\n",
    "Step 1:\n",
    "To establish Minkowski's inequality for sums, we'll employ Hölder's inequality. Hölder's inequality states that for any two sequences of real numbers $(x_k)$ and $(y_k)$ and any $p>1$ such that $\\frac{1}{p} + \\frac{1}{q} = 1$, the following holds:\n",
    "\n",
    "$\\sum_{k=1}^n |x_k y_k| \\leq \\left( \\sum_{k=1}^n |x_k|^p \\right)^{\\frac{1}{p}} \\left( \\sum_{k=1}^n |y_k|^q \\right)^{\\frac{1}{q}}$\n",
    "\n",
    "Step 2:\n",
    "Now, let's define $x_k = \\frac{|a_k|^p}{\\left(\\sum_{k=1}^n |a_k|^p\\right)^{\\frac{1}{p}}}$ and $y_k = \\frac{|b_k|^p}{\\left(\\sum_{k=1}^n |b_k|^p\\right)^{\\frac{1}{p}}}$. \n",
    "\n",
    "Step 3:\n",
    "Then, we have:\n",
    "\n",
    "\\begin{align*}\n",
    "\\sum_{k=1}^n |a_k + b_k|^p &= \\sum_{k=1}^n |a_k + b_k|^p \\cdot 1^{1-p} \\\\\n",
    "&\\leq \\left( \\sum_{k=1}^n |a_k|^p \\right)^{\\frac{1}{p}} \\left( \\sum_{k=1}^n |b_k|^p \\right)^{\\frac{1}{q}} \\left( \\sum_{k=1}^n 1^{q} \\right)^{1/q} \\\\\n",
    "&= \\left( \\sum_{k=1}^n |a_k|^p \\right)^{\\frac{1}{p}} \\left( \\sum_{k=1}^n |b_k|^p \\right)^{\\frac{1}{p}} \\left( \\sum_{k=1}^n 1 \\right)^{1/q} \\\\\n",
    "&= \\left( \\sum_{k=1}^n |a_k|^p \\right)^{\\frac{1}{p}} \\left( \\sum_{k=1}^n |b_k|^p \\right)^{\\frac{1}{p}} n^{1/q}\n",
    "\\end{align*}\n",
    "\n",
    "Given $\\frac{1}{p} + \\frac{1}{q} = 1$, we find $q = \\frac{p}{p-1}$.\n",
    "\n",
    "Thus, $n^{1/q} = n^{\\frac{p-1}{p}} = n^{\\frac{1}{p-1}}$.\n",
    "\n",
    "Hence:\n",
    "\n",
    "$\\sum_{k=1}^n |a_k + b_k|^p \\leq \\left( \\sum_{k=1}^n |a_k|^p \\right)^{\\frac{1}{p}} \\left( \\sum_{k=1}^n |b_k|^p \\right)^{\\frac{1}{p}} n^{\\frac{1}{p-1}}$\n",
    "\n",
    "Step 4:\n",
    "Dividing both sides by $n^{\\frac{1}{p-1}}$:\n",
    "\n",
    "$\\frac{1}{n^{\\frac{1}{p-1}}} \\sum_{k=1}^n |a_k + b_k|^p \\leq \\left( \\sum_{k=1}^n |a_k|^p \\right)^{\\frac{1}{p}} \\left( \\sum_{k=1}^n |b_k|^p \\right)^{\\frac{1}{p}}$\n",
    "\n",
    "Step 5:\n",
    "Taking the $p$-th root on both sides:\n",
    "\n",
    "$\\left( \\frac{1}{n} \\sum_{k=1}^n |a_k + b_k|^p \\right)^{\\frac{1}{p}} \\leq \\left( \\sum_{k=1}^n |a_k|^p \\right)^{\\frac{1}{p}} \\left( \\sum_{k=1}^n |b_k|^p \\right)^{\\frac{1}{p}}$\n",
    "\n",
    "<br>\n",
    "\n",
    "**Thus, Minkowski's inequality for sums is established.**\n",
    "<br><br>\n",
    "****"
   ]
  },
  {
   "cell_type": "markdown",
   "metadata": {},
   "source": [
    "*3. Prove the triangle inequality $|x+y| \\leq |x| + |y|, \\forall (x,y) \\in \\mathbb{R}$*\n",
    "<br><br>\n",
    "\n",
    "**ANSWER:**\n",
    "\n",
    "Step 1:\n",
    "\n",
    "To prove the triangle inequality $|x+y| \\leq |x| + |y|$, we can consider the cases where $x$ and $y$ are both positive, both negative, or of opposite signs.\n",
    "\n",
    "Step 2:\n",
    "\n",
    "Case 1: $x$ and $y$ are both positive:\n",
    "$|x+y| = x+y$ \n",
    "$|x| + |y| = x + y$ \n",
    "In this case, since $x$ and $y$ are both positive, their absolute values are the same as the original values. So $|x+y| = |x| + |y|$ holds true.\n",
    "\n",
    "Step 3:\n",
    "\n",
    "Case 2: $x$ and $y$ are both negative:\n",
    "$|x+y| = -(x+y) = -x - y$ \n",
    "$|x| + |y| = -x - y$ \n",
    "In this case, since $x$ and $y$ are both negative, their absolute values are the negations of the original values. So $|x+y| = |x| + |y|$ holds true.\n",
    "\n",
    "Step 4:\n",
    "\n",
    "Case 3: $x$ and $y$ have opposite signs:\n",
    "Without loss of generality, assume $x > 0$ and $y < 0$. Then,\n",
    "$|x+y| = |x-y|$ \n",
    "$|x| + |y| = x + (-y) = x - y$ \n",
    "Since $x > y$ (because $x$ is positive and $y$ is negative), $|x-y| = x-y$, so $|x+y| = |x| + |y|$ holds true.\n",
    "\n",
    "Step 5:\n",
    "<br>\n",
    "\n",
    "**In all cases, we have shown that $|x+y| \\leq |x| + |y|$, thus proving the triangle inequality for all real numbers $x$ and $y$.**\n",
    "<br><br>\n",
    "\n",
    "****"
   ]
  },
  {
   "cell_type": "markdown",
   "metadata": {},
   "source": [
    "*4. Prove Sedrakayan's Lemma $\\forall u_i, v_i \\in \\mathbb{R}^+$:*\n",
    "\n",
    "\\begin{gather}\n",
    "\\frac{(\\sum_{i=1}^n u_i)^2}{\\sum_{i=1}^n v_i}\n",
    "\\leq\n",
    "\\sum_{i=1}^n \\frac{(u_i)^2}{v_i}\n",
    "\\end{gather}*\n",
    "\n",
    "<br><br>\n",
    "**ANSWER:**\n",
    "\n",
    "Step 1:\n",
    "\n",
    "We aim to prove Sedrakayan's Lemma, which asserts:\n",
    "\n",
    "For any positive real numbers $u_i$ and $v_i$ (where $i$ ranges from 1 to $n$):\n",
    "\n",
    "$\\frac{(\\sum_{i=1}^n u_i)^2}{\\sum_{i=1}^n v_i} \\leq \\sum_{i=1}^n \\frac{u_i^2}{v_i}$\n",
    "\n",
    "To establish this, we'll utilize the Cauchy-Schwarz Inequality.\n",
    "\n",
    "Step 2:\n",
    "\n",
    "Define two vectors:\n",
    "   - $\\mathbf{u} = (u_1, u_2, ..., u_n)$\n",
    "   - $\\mathbf{v} = (\\sqrt{v_1}, \\sqrt{v_2}, ..., \\sqrt{v_n})$\n",
    "\n",
    "Step 3:\n",
    "\n",
    "Next, we utilize the Cauchy-Schwarz Inequality for inner products of vectors. This inequality asserts that the square of the dot product of two vectors is smaller than or equal to the product of the squares of their magnitudes.\n",
    "\n",
    "Step 4:\n",
    "\n",
    "For the sum of $u_i$, we have:\n",
    "$(\\sum_{i=1}^n u_i)^2 \\leq n (\\sum_{i=1}^n u_i^2)$\n",
    "\n",
    "For the sum of $\\sqrt{v_i}$, we have:\n",
    "$(\\sum_{i=1}^n \\sqrt{v_i})^2 \\leq n (\\sum_{i=1}^n v_i)$\n",
    "\n",
    "Step 5:\n",
    "\n",
    "3. Rearranging, we obtain:\n",
    "$\\frac{(\\sum_{i=1}^n u_i)^2}{\\sum_{i=1}^n v_i} \\leq \\frac{\\sum_{i=1}^n u_i^2}{n}$\n",
    "\n",
    "Step 6:\n",
    "\n",
    "Now, we know that $\\mathbf{u} \\cdot \\mathbf{v} \\leq |\\mathbf{u}| \\cdot |\\mathbf{v}|$. Expanding the dot product:\n",
    "$\\sum_{i=1}^n u_i \\sqrt{v_i} \\leq \\sqrt{\\sum_{i=1}^n u_i^2} \\sqrt{\\sum_{i=1}^n v_i}$\n",
    "\n",
    "Step 7:\n",
    "\n",
    "Square both sides:\n",
    "$(\\sum_{i=1}^n u_i \\sqrt{v_i})^2 \\leq (\\sum_{i=1}^n u_i^2)(\\sum_{i=1}^n v_i)$\n",
    "\n",
    "Step 8:\n",
    "\n",
    "Substitute back $\\mathbf{u} = (u_1, u_2, ..., u_n)$ and $\\mathbf{v} = (\\sqrt{v_1}, \\sqrt{v_2}, ..., \\sqrt{v_n})$:\n",
    "$\\left(\\sum_{i=1}^n u_i \\sqrt{v_i}\\right)^2 \\leq \\left(\\sum_{i=1}^n u_i^2\\right) \\left(\\sum_{i=1}^n v_i\\right)$\n",
    "\n",
    "Step 9:\n",
    "\n",
    "Rearranging, we obtain:\n",
    "$\\frac{(\\sum_{i=1}^n u_i)^2}{\\sum_{i=1}^n v_i} \\leq \\sum_{i=1}^n \\frac{u_i^2}{v_i}$\n",
    "\n",
    "<br>\n",
    "\n",
    "This validates **Sedrakayan's Lemma**."
   ]
  },
  {
   "cell_type": "markdown",
   "metadata": {},
   "source": [
    "****\n",
    "### More Problems\n",
    "\n",
    "1. Consider the functions $f(x) = 2x+1$, $g(x) = 2y-1$, $j(x) = |f(x)+g(x)|$, and $h(x) = j(x)^2$.\n",
    "\n",
    "Show for the following inequality that:\n",
    "\n",
    "$ \\sqrt{|f(x)|^2} \\geq \\sqrt{h(x)} - \\sqrt{|g(x)|^2}, \\forall (x,y) \\in \\mathbb{Z}^+ $\n",
    "\n",
    "**Solution:**\n",
    "\n",
    "Step 1:\n",
    "\n",
    " **Calculate $|f(x)|^2$**:\n",
    "    $|f(x)|^2 = |2x+1|^2 = (2x+1)^2$\n",
    "   \n",
    "Here, we compute the squared magnitude of the function $f(x)$. Since $f(x)$ is a linear function, squaring it results in $(2x+1)^2$.\n",
    "\n",
    "Step 2:\n",
    "\n",
    " **Calculate $|g(x)|^2$**:\n",
    "    $|g(x)|^2 = |2y-1|^2 = (2y-1)^2$\n",
    "    \n",
    "Similarly, we compute the squared magnitude of the function $g(x)$. Squaring $g(x)$ results in $(2y-1)^2$.\n",
    "\n",
    "Step 3:\n",
    "\n",
    " **Calculate $j(x)$**:\n",
    "    $j(x) = |f(x) + g(x)| = |(2x+1) + (2y-1)| = |2x + 1 + 2y - 1| = |2x + 2y| = 2|x + y|$\n",
    "    \n",
    "We find $j(x)$ by adding $f(x)$ and $g(x)$ and taking the absolute value. Simplifying inside the absolute value, we get $2|x + y|$ because $2x + 2y$ is always positive for positive integers $x$ and $y$.\n",
    "\n",
    "Step 4:\n",
    "\n",
    " **Calculate $h(x)$**:\n",
    "    $h(x) = j(x)^2 = (2|x + y|)^2 = 4(x + y)^2$\n",
    "    \n",
    "We square the function $j(x)$. Since $j(x) = 2|x + y|$, squaring it results in $4(x + y)^2$.\n",
    "\n",
    "Step 5:\n",
    "\n",
    " **Calculate $\\sqrt{h(x)}$**:\n",
    "   $\\sqrt{h(x)} = \\sqrt{4(x + y)^2} = 2|x + y|$\n",
    "    \n",
    "Taking the square root of $h(x)$, we get back to $2|x + y|$ because the square root and the square cancel out.\n",
    "\n",
    "Step 6:\n",
    "\n",
    " **Express the inequality**:\n",
    "    $\\sqrt{|f(x)|^2} \\geq \\sqrt{h(x)} - \\sqrt{|g(x)|^2}$\n",
    "   \n",
    "The given inequality is written in terms of the square roots of the squared magnitudes of $f(x)$ and $g(x)$, and the square root of $h(x)$.\n",
    "\n",
    "Step 7:\n",
    "\n",
    " **Substitute the expressions**:\n",
    "   $\\sqrt{(2x+1)^2} \\geq 2|x+y| - \\sqrt{(2y-1)^2}$\n",
    "    \n",
    "Substituting the expressions calculated earlier into the inequality, we get $\\sqrt{(2x+1)^2}$ for $|f(x)|^2$, $2|x + y|$ for $\\sqrt{h(x)}$, and $\\sqrt{(2y-1)^2}$ for $|g(x)|^2$.\n",
    "\n",
    "Step 8:\n",
    "\n",
    " **Simplify the square roots**:\n",
    "    $|2x+1| \\geq 2|x+y| - |2y-1|$\n",
    "    \n",
    "Simplifying the square roots of the squared terms, we get $|2x+1|$ and $|2y-1|$. Since these are positive values (for $x, y \\in \\mathbb{Z}^+$), the absolute values can be removed.\n",
    "\n",
    "Step 9:\n",
    "\n",
    " **Consider the properties of absolute values**:\n",
    "   \n",
    "Since $x, y \\in \\mathbb{Z}^+$, $2x+1$ and $2y-1$ are positive, so the absolute values can be removed:\n",
    "   \n",
    "   $2x+1 \\geq 2(x+y) - (2y-1)$\n",
    "   \n",
    "For positive integers $x$ and $y$, $2x+1$ and $2y-1$ are always positive, so the absolute values can be removed safely.\n",
    "\n",
    "Step 10:\n",
    "\n",
    " **Simplify the inequality**:\n",
    "    $2x+1 \\geq 2x + 2y - 2y + 1$\n",
    "   \n",
    "Simplifying the right-hand side of the inequality:\n",
    "    $2x+1 \\geq 2x+1$\n",
    "   \n",
    "After simplifying, we see that the inequality $2x + 1 \\geq 2x + 1$ holds true.\n",
    "\n",
    "Step 11:\n",
    "\n",
    " **Conclusion**:\n",
    "The inequality $2x+1 \\geq 2x+1$ holds true for all $x, y \\in \\mathbb{Z}^+$.\n",
    "   \n",
    "This shows that the original inequality is always satisfied for positive integers $x$ and $y$.\n",
    "\n",
    "### Final Conclusion:\n",
    "\n",
    "**Therefore, we have shown that:**\n",
    "$\\sqrt{|f(x)|^2} \\geq \\sqrt{h(x)} - \\sqrt{|g(x)|^2}, \\forall (x,y) \\in \\mathbb{Z}^+$"
   ]
  },
  {
   "cell_type": "markdown",
   "metadata": {},
   "source": [
    "****\n",
    "\n",
    "2. Prove Sedrakayan's Lemma if $ u_i $ and $ v_i $ are square roots of an even integers\n",
    "\n",
    "$\n",
    "\\frac{(\\sum_{i=1}^n u_i)^2}{\\sum_{i=1}^n v_i} \\leq \\sum_{i=1}^n \\frac{u_i^2}{v_i}\n",
    "$\n",
    "\n",
    "**Solution:**\n",
    "\n",
    "Step 1:\n",
    "\n",
    " **Restate the Lemma**:\n",
    "   We want to show:\n",
    "   $\n",
    "   \\frac{\\left(\\sum_{i=1}^n u_i\\right)^2}{\\sum_{i=1}^n v_i} \\leq \\sum_{i=1}^n \\frac{u_i^2}{v_i}\n",
    "   $\n",
    "\n",
    "Step 2:\n",
    "\n",
    " **Cauchy-Schwarz Inequality**:\n",
    "   Recall the Cauchy-Schwarz inequality in the form:\n",
    "   $\n",
    "   \\left( \\sum_{i=1}^n a_i b_i \\right)^2 \\leq \\left( \\sum_{i=1}^n a_i^2 \\right) \\left( \\sum_{i=1}^n b_i^2 \\right)\n",
    "   $\n",
    "\n",
    "Step 3:\n",
    "\n",
    " **Define Sequences**:\n",
    "   Let:\n",
    "   $\n",
    "   a_i = \\frac{u_i}{\\sqrt{v_i}} \\quad \\text{and} \\quad b_i = \\sqrt{v_i}\n",
    "   $\n",
    "\n",
    "Step 4:\n",
    "\n",
    " **Apply Cauchy-Schwarz**:\n",
    "   Applying the Cauchy-Schwarz inequality:\n",
    "   $\n",
    "   \\left( \\sum_{i=1}^n \\frac{u_i}{\\sqrt{v_i}} \\cdot \\sqrt{v_i} \\right)^2 \\leq \\left( \\sum_{i=1}^n \\left( \\frac{u_i}{\\sqrt{v_i}} \\right)^2 \\right) \\left( \\sum_{i=1}^n (\\sqrt{v_i})^2 \\right)\n",
    "   $\n",
    "\n",
    "Step 5:\n",
    "\n",
    " **Simplify the Left-Hand Side**:\n",
    "   The left-hand side simplifies to:\n",
    "   $\n",
    "   \\left( \\sum_{i=1}^n u_i \\right)^2\n",
    "   $\n",
    "\n",
    "Step 6:\n",
    "\n",
    " **Simplify the Right-Hand Side**:\n",
    "   The right-hand side simplifies to:\n",
    "   $\n",
    "   \\left( \\sum_{i=1}^n \\frac{u_i^2}{v_i} \\right) \\left( \\sum_{i=1}^n v_i \\right)\n",
    "   $\n",
    "\n",
    "Step 7:\n",
    "\n",
    " **Combine the Results**:\n",
    "   From the previous steps, we have:\n",
    "   $\n",
    "   \\left( \\sum_{i=1}^n u_i \\right)^2 \\leq \\left( \\sum_{i=1}^n \\frac{u_i^2}{v_i} \\right) \\left( \\sum_{i=1}^n v_i \\right)\n",
    "   $\n",
    "\n",
    "Step 8:\n",
    "\n",
    " **Divide Both Sides**:\n",
    "   Divide both sides by $\\sum_{i=1}^n v_i$:\n",
    "   $\n",
    "   \\frac{\\left( \\sum_{i=1}^n u_i \\right)^2}{\\sum_{i=1}^n v_i} \\leq \\sum_{i=1}^n \\frac{u_i^2}{v_i}\n",
    "   $\n",
    "\n",
    "### Final Conclusion\n",
    "\n",
    "Thus, we have shown that:\n",
    "\n",
    "$\n",
    "\\frac{\\left( \\sum_{i=1}^n u_i \\right)^2}{\\sum_{i=1}^n v_i} \\leq \\sum_{i=1}^n \\frac{u_i^2}{v_i}\n",
    "$\n",
    "\n",
    "**This confirms that the inequality holds, completing the proof of Sedrakayan's Lemma.**"
   ]
  }
 ],
 "metadata": {
  "kernelspec": {
   "display_name": "base",
   "language": "python",
   "name": "python3"
  },
  "language_info": {
   "codemirror_mode": {
    "name": "ipython",
    "version": 3
   },
   "file_extension": ".py",
   "mimetype": "text/x-python",
   "name": "python",
   "nbconvert_exporter": "python",
   "pygments_lexer": "ipython3",
   "version": "3.12.3"
  }
 },
 "nbformat": 4,
 "nbformat_minor": 2
}
