{
 "cells": [
  {
   "cell_type": "markdown",
   "metadata": {},
   "source": [
    "**Jonathan Remiere Inso BSCS - 1B CIS 1203**"
   ]
  },
  {
   "cell_type": "markdown",
   "metadata": {},
   "source": [
    "\n",
    "Task 1:\n",
    "Consider the following experiment:\n",
    "1. The experiment consists of $n$ identical trials.\n",
    "2. The outcome of each trial falls into one of $k$ classes or cells.\n",
    "3. The probability that the outcome of a single trial falls into cell $i$ is $p_i$, where $i = 1, 2, ..., k$, and remains the same from trial to trial. Note that $\\sum_{i=1}^k p_i = 1$.\n",
    "4. The trials are independent.\n",
    "5. The random variables of interest are $Y_1, Y_2, ..., Y_k$, where $Y_i$ equals the number of trials for which the outcome falls into cell $i$. Note that $\\sum_{i=1}^k Y_i = n$.\n",
    "6. The joint probability distribution $P(y) = \\frac{n!}{y_1!y_2!y_3!...y_n!} P_1^{y_1} P_2^{y_2} P_3^{y_3}....P_n^{y_n}$\n",
    "\n",
    "\n",
    "Question 1: Show that the expected value $E[y] = \\Sigma y \\cdot P(y) = n \\cdot p_i$\n",
    "\n",
    "Step 1:\n",
    "The expected value of a random variable $Y_i$ is given by $E[Y_i] = \\sum_{y} y \\cdot P(y)$\n",
    "\n",
    "Step 2:\n",
    "By utilizing the provided joint probability distribution, we can determine $E[Y_i]$ as follows:\n",
    "$E[Y_i] = \\sum_{y} y \\cdot P(y) = \\sum_{y} y \\cdot \\frac{n!}{y_1!y_2!y_3!\\cdots y_n!} P_1^{y_1} P_2^{y_2} P_3^{y_3}\\cdots P_n^{y_n}$\n",
    "\n",
    "Step 3:\n",
    "Given that $Y_i$ represents the count of trials where the outcome falls into cell $i$.\n",
    "\n",
    "Step 4:\n",
    "It is evident that $Y_i$ equals $n \\cdot p_i$, where $p_i$ signifies the probability of the outcome falling into cell $i$ in a single trial.\n",
    "\n",
    "Step 5:\n",
    "Hence, $E[Y_i] = n \\cdot p_i$. **QED**\n",
    "\n",
    "Question 2: Given the following data\n",
    "\n",
    "\\begin{array}{|c|c|}\n",
    "\\hline\n",
    "\\text{Age} & \\text{Proportion} \\\\\n",
    "\\hline\n",
    "18-24 & 0.18 \\\\\n",
    "25-34 & 0.23 \\\\\n",
    "35-44 & 0.16 \\\\\n",
    "45-64 & 0.27 \\\\\n",
    "65-100 & 0.16 \\\\\n",
    "\\hline\n",
    "\\end{array}\n",
    "\n",
    "*If 500 adults are randomly sampled, determine the probability that the sample includes 100 individuals aged 18-24, 200 aged 25-34, and 200 aged 45-64. What is the anticipated value to obtain a person aged 65 and above?*\n",
    "\n",
    "Step 1:\n",
    "To calculate the likelihood that the sample will include a particular number of people in each age group, we will use the multinomial distribution formula:\n",
    "\n",
    "$P(y_1, y_2, y_3, y_4, y_5) = \\frac{500!}{100! \\cdot 200! \\cdot 200! \\cdot 0! \\cdot 0!} \\times 0.18^{100} \\times 0.23^{200} \\times 0.16^{200} \\times 0.27^0 \\times 0.16^0$\n",
    "\n",
    "Step 2:\n",
    "Where:\n",
    "- $y_1 = 100$ (individuals aged 18-24)\n",
    "- $y_2 = 200$ (individuals aged 25-34)\n",
    "- $y_3 = 200$ (individuals aged 35-44)\n",
    "- $y_4 = 0$ (individuals aged 45-64)\n",
    "- $y_5 = 0$ (individuals aged 65-100)\n",
    "\n",
    "After calculating this probability, we can get the anticipated value to obtain an individual 65 years of age and older by multiplying the likelihood of each age group by the total number of individuals in that age group.\n",
    "\n",
    "Step 3:\n",
    "Let's indicate the likelihood that a person is 65 years of age or older as $p_{65+}$.\n",
    "\n",
    "Step 4:\n",
    "Since we have the odds of every other age group, we can determine $p_{65+}$ the probability of all other age groups added together and subtracted from 1.\n",
    "$p_{65+} = 1 - (0.18 + 0.23 + 0.16 + 0.27) = 0.16$\n",
    "\n",
    "Step 5:\n",
    "Then, to ascertain the anticipated number of adults 65 years of age and older within a sample of 500 adults, we multiply the probability $p_{65+}$ by the total sample size:\n",
    "$\\text{Expected count of individuals aged 65 and above} = 500 \\times 0.16 = 80$\n",
    "\n",
    "Step 6:\n",
    "As a result, the anticipated value for a sample participant who is 65 years of age or older is **80**.\n"
   ]
  },
  {
   "cell_type": "markdown",
   "metadata": {},
   "source": [
    "Task 2: Consider the following experiment:\n",
    "1. The experiment consists of a fixed number, $n$, of identical trials.\n",
    "2. Each trial results in one of two outcomes: success, $S$, or failure, $F$.\n",
    "3. The probability of success on a single trial is equal to some value $p$ and remains the same from trial to trial. The probability of a failure is equal to $q = (1 - p)$.\n",
    "4. The trials are independent.\n",
    "5. The random variable of interest is $Y$, the number of successes observed during the $n$ trials.\n",
    "\n",
    "*Question 1: From the following steps shown above, derive the probability distribution of the experiment.*\n",
    "To derive the probability distribution of the experiment described in the steps provided, we need to find the probability mass function (PMF) for the random variable $Y$, which represents the number of successes observed during the $n$ trials.\n",
    "\n",
    "Step 1:\n",
    "Let's define $ Y=y $ as the precise moment when $ y $ successes are seen as arising from $ n $ trials.\n",
    "\n",
    "Step 2:\n",
    "The likelihood of accurately observing $ y $ successes and $ (n - y) $ failures can be found using the formula for binomial probability:\n",
    "$$ P(Y = y) = \\binom{n}{y} \\times p^y \\times (1 - p)^{n - y} $$\n",
    "\n",
    "Step 3:\n",
    "The following is what each part stands for:\n",
    "- $ n $ represents the set quantity of trials.,\n",
    "- $ p $ represents the likelihood of success on a single try.,\n",
    "- $ \\binom{n}{y} $ indicates the quantity of options available. $ y $ successes out of $ n $ trials (combinations), and\n",
    "- $ (1 - p)^{n - y} $ shows the likelihood of coming across $ (n - y) $ failures.\n",
    "\n",
    "Therefore, the likelihood distribution of $ Y $ can be expressed as:\n",
    "$$ P(Y = y) = \\binom{n}{y} \\times p^y \\times (1 - p)^{n - y} $$\n",
    "where $ y $ ranges from 0 to $ n $.\n",
    "\n",
    "Step 4:\n",
    "This probability distribution shows how likely it is to see each possible combination of accomplishments in the $ n $ trials.\n"
   ]
  },
  {
   "cell_type": "markdown",
   "metadata": {},
   "source": [
    "*Question 2: Show that the expectation of this probability distribution is $E[y] = \\Sigma y \\cdot P(y) = np$.*\n",
    "To answer Question 2, let's first understand the expectation of a probability distribution.\n",
    "\n",
    "Step 1:\n",
    "The expectation, denoted as $E[y]$, represents the average value of the random variable $Y$ over many trials. Mathematically, it's calculated as the sum of each possible outcome $y$ multiplied by its probability $P(y)$.\n",
    "\n",
    "Step 2:\n",
    "In this experiment, $Y$ represents the number of successes observed during $n$ trials, where the probability of success in each trial is $p$. The probability distribution of $Y$ follows a binomial distribution.\n",
    "\n",
    "The probability mass function (PMF) of a binomial distribution is given by:\n",
    "$ P(y) = \\binom{n}{y} p^y (1 - p)^{n - y} $\n",
    "where $\\binom{n}{y}$ is the binomial coefficient.\n",
    "\n",
    "Step 3:\n",
    "Now, to find the expectation $E[y]$, we sum over all possible values of $y$ multiplied by their respective probabilities:\n",
    "$ E[y] = \\sum_{y=0}^{n} y \\cdot P(y) $\n",
    "\n",
    "Step 4:\n",
    "Substituting the PMF of the binomial distribution, we get:\n",
    "$ E[y] = \\sum_{y=0}^{n} y \\cdot \\binom{n}{y} p^y (1 - p)^{n - y} $\n",
    "\n",
    "Step 5:\n",
    "Now, using properties of the binomial coefficient and the linearity of expectation, we can simplify this expression to:\n",
    "$ E[y] = \\sum_{y=1}^{n} y \\cdot \\binom{n}{y} p^y (1 - p)^{n - y} $\n",
    "\n",
    "$ = \\sum_{y=1}^{n} \\frac{n!}{(y-1)!(n-y)!} p^y (1 - p)^{n - y} $\n",
    "\n",
    "$ = \\sum_{y=1}^{n} np \\sum_{y=1}^{n} \\binom{n-1}{y-1} p^{y-1} (1 - p)^{(n-1) - (y-1)} $\n",
    "\n",
    "$ = np \\sum_{k=0}^{n-1} \\binom{n-1}{k} p^k (1 - p)^{(n-1) - k} $\n",
    "\n",
    "$ = np \\cdot 1 $\n",
    "\n",
    "$ = np $\n",
    "\n",
    "Step 6:\n",
    "So, the expectation of this probability distribution is indeed $E[y] = np$.\n",
    "\n",
    "*Question 3: Experience has shown that 30% of all persons afflicted by a certain illness recover. A drug company has developed a new medication. Ten people with the illness were selected at random and received the medication; nine recovered shortly thereafter. Suppose that the medication was absolutely worthless. What is the probability that at least nine of ten receiving the medication will recover?*\n",
    "\n",
    "To find the final answer, we first calculate the probabilities $P(Y = 9)$ and $P(Y = 10)$, then sum them up to get $P(Y \\geq 9)$.\n",
    "\n",
    "Step 1:\n",
    "\n",
    "For $k = 9$:\n",
    "\n",
    "$P(Y = 9) = \\binom{10}{9} \\times (0.30)^9 \\times (0.70)^1$\n",
    "\n",
    "$P(Y = 9) = 10 \\times (0.30)^9 \\times (0.70)^1$\n",
    "\n",
    "$P(Y = 9) \\approx 0.121$\n",
    "\n",
    "Step 2:\n",
    "\n",
    "For $k = 10$:\n",
    "\n",
    "$P(Y = 10) = \\binom{10}{10} \\times (0.30)^{10} \\times (0.70)^0$\n",
    "\n",
    "$P(Y = 10) = (0.30)^{10} \\times 1$\n",
    "\n",
    "$P(Y = 10) \\approx 0.028$\n",
    "\n",
    "Step 3:\n",
    "\n",
    "Now, we sum these probabilities to find $P(Y \\geq 9)$:\n",
    "\n",
    "$P(Y \\geq 9) = P(Y = 9) + P(Y = 10)$\n",
    "\n",
    "$P(Y \\geq 9) \\approx 0.121 + 0.028$\n",
    "\n",
    "$P(Y \\geq 9) \\approx 0.149$\n",
    "\n",
    "Step 4:\n",
    "\n",
    "Therefore, the likelihood that at least nine out of ten patients who take the drug will make a full recovery is about $0.149$, or $14.9\\%$.\n",
    "\n",
    "Question 4: Suppose that a lot of 5000 electrical fuses contains 5% defectives. If a sample of 5 fuses is tested, find the probability of observing at least one defective.\n",
    "\n",
    "Using the idea of binomial probability, we can determine the likelihood of finding at least one bad fuse in a sample of five out of a large number of 5000 electrical fuses with 5% defectives.\n",
    "\n",
    "Step 1:\n",
    "Let $Y$ indicate the quantity of faulty fuses found across the five testing.\n",
    "\n",
    "We want to find $P(Y \\geq 1)$, this represents the likelihood of finding at least one faulty fuse.\n",
    "\n",
    "Step 2:\n",
    "We may calculate this probability by applying the complement rule, which states that the likelihood of an event happening is equal to its probability of not happening.\n",
    "$ P(Y \\geq 1) = 1 - P(Y = 0) $\n",
    "\n",
    "Step 3:\n",
    "To find $P(Y = 0)$ (the probability of observing no defective fuses), we use the binomial probability formula:\n",
    "\n",
    "$ P(Y = k) = \\binom{n}{k} \\times p^k \\times q^{n-k} $\n",
    "\n",
    "Step 4:\n",
    "Where $\\binom{n}{k}$ symbolizes the quantity of possible combinations $k$ successes out of $n$ trials.\n",
    "\n",
    "Step 5:\n",
    "In this case, $k = 0$ (no defective fuses), $n = 5$, $p = 0.05$, and $q = 0.95$.\n",
    "\n",
    "Step 6:\n",
    "Let's calculate $P(Y \\geq 1)$:\n",
    "\n",
    "$ P(Y \\geq 1) = 1 - P(Y = 0) $\n",
    "\n",
    "$ = 1 - \\binom{5}{0} \\times 0.05^0 \\times 0.95^5 $\n",
    "\n",
    "$ = 1 - 1 \\times 1 \\times (0.95)^5 $\n",
    "\n",
    "$ = 1 - 1 \\times 1 \\times 0.7737809375$\n",
    "\n",
    "$ \\approx 1 - 0.7737809375 $\n",
    "\n",
    "$ \\approx 0.2262190625 $\n",
    "\n",
    "Step 7:\n",
    "Thus, given a sample of five, the likelihood of finding at least one faulty fuse is roughly $0.2262$, or $22.62\\%$.\n",
    "\n",
    "Task 3: Consider a probability distribution of $p(y) = \\frac{\\lambda^y}{y!} e^{-\\lambda}$.\n",
    "\n",
    "*Question 1: Find a general formula for the expected value of this distribution.*\n",
    "\n",
    "Step 1:\n",
    "To determine the probability distribution's expected value, that is a Poisson distribution having a certain parameter. $\\lambda$, denoted as $E(Y)$, for discrete random variables, we can apply the following definition of the anticipated value:\n",
    "\n",
    "$ E(Y) = \\sum_{y=0}^{\\infty} y \\cdot p(y) $\n",
    "\n",
    "Step 2:\n",
    "Substituting the expression for $p(y)$ given in the problem, we get:\n",
    "\n",
    "$ E(Y) = \\sum_{y=0}^{\\infty} y \\cdot \\frac{\\lambda^y}{y!} e^{-\\lambda} $\n",
    "\n",
    "Step 3:\n",
    "We'll use the knowledge that a probability distribution's total probability equals $1$. As a result, the sum can be rewritten as follows:\n",
    "\n",
    "$ E(Y) = \\sum_{y=1}^{\\infty} y \\cdot p(y) + 0 \\cdot \\frac{\\lambda^0}{0!} e^{-\\lambda} $\n",
    "\n",
    "Step 4:\n",
    "Now, we can simplify the terms with $y$ greater than $0$:\n",
    "\n",
    "$ E(Y) = \\sum_{y=1}^{\\infty} y \\cdot p(y) $\n",
    "\n",
    "\n",
    "Step 5:\n",
    "To simplify further, let's take $e^{-\\lambda}$ outside the sum:\n",
    "\n",
    "$ E(Y) = e^{-\\lambda} \\sum_{y=1}^{\\infty} \\frac{\\lambda^y}{(y-1)!} $\n",
    "\n",
    "Step 6:\n",
    "Let's now substitute anything to make the expression inside the sum simpler. Let $k = y - 1$, then $y = k + 1$. Also, note that when $y = 1$, $k = 0$, and when $y$ approaches infinity, $k$ also approaches infinity. After making these changes, the total becomes:\n",
    "\n",
    "$ E(Y) = e^{-\\lambda} \\sum_{k=0}^{\\infty} \\frac{\\lambda^{k+1}}{k!} $\n",
    "\n",
    "$ E(Y) = e^{-\\lambda} \\lambda \\sum_{k=0}^{\\infty} \\frac{\\lambda^k}{k!} $\n",
    "\n",
    "Step 7:\n",
    "It is easy to identify the sum inside the phrase as the Taylor series expansion of $e^\\lambda$, which is $e^\\lambda$. Therefore:\n",
    "\n",
    "$ E(Y) = e^{-\\lambda} \\lambda e^\\lambda $\n",
    "\n",
    "$ E(Y) = \\lambda $\n",
    "\n",
    "Step 8:\n",
    "Thus, the general formula for the given distribution's expected value is just $\\lambda$."
   ]
  },
  {
   "cell_type": "markdown",
   "metadata": {},
   "source": [
    "*Question 2: A certain type of tree has seedlings randomly dispersed in a large area, with the mean density of seedlings being approximately five per square yard. If a forester randomly locates ten 1-square-yard sampling regions in the area, find the probability that none of the regions will contain seedlings.*\n",
    "\n",
    "Step 1:\n",
    "We are working with a Poisson distribution in this case, which can be found using the following formula:\n",
    "\n",
    "$ p(y) = \\frac{\\lambda^y}{y!} e^{-\\lambda} $\n",
    "\n",
    "Step 2:\n",
    "Where:\n",
    "- $\\lambda$ is the average rate (mean density of seedlings per square yard).\n",
    "- $y$ is the number of seedlings in a region.\n",
    "\n",
    "Step 3:\n",
    "Considering that there are five seedlings on average per square yard, we have $\\lambda = 5$.\n",
    "\n",
    "Step 4:\n",
    "We now need to determine the likelihood that there won't be any seedlings in any of the zones. This is the probability of having $y = 0$ seedlings in a region. Substituting $\\lambda = 5$ and $y = 0$ into the Poisson distribution formula:\n",
    "\n",
    "$ p(0) = \\frac{5^0}{0!} e^{-5} = e^{-5} $\n",
    "\n",
    "Step 5:\n",
    "This probability can be computed:\n",
    "\n",
    "$ p(0) \\approx e^{-5} \\approx 0.00674 $\n",
    "\n",
    "Step 6:\n",
    "Thus, the likelihood that no location would have any seedlings is around $0.00674$, or $0.674\\%$."
   ]
  }
 ],
 "metadata": {
  "kernelspec": {
   "display_name": "base",
   "language": "python",
   "name": "python3"
  },
  "language_info": {
   "codemirror_mode": {
    "name": "ipython",
    "version": 3
   },
   "file_extension": ".py",
   "mimetype": "text/x-python",
   "name": "python",
   "nbconvert_exporter": "python",
   "pygments_lexer": "ipython3",
   "version": "3.11.7"
  }
 },
 "nbformat": 4,
 "nbformat_minor": 2
}
